\documentclass{article}

\usepackage{amsmath}

\begin{document}
	
	\title{Following Two Mathematical Equations}
	\date{}
	\maketitle
	
	\[
	\begin{aligned}
		x &= \frac{-b \pm \sqrt{b^2 - 4ac}}{2a} \\
		&= \frac{-2 \pm \sqrt{2^2 - 4 \cdot 1 \cdot (-8)}}{2 \cdot 1} \\
		&= \frac{-2 \pm \sqrt{4 + 32}}{2}
	\end{aligned}
	\quad \quad \quad
	\begin{aligned}
		\varphi_{\sigma}^{\lambda} A_{t} &= \sum_{\pi \in C_{t}} \operatorname{sgn}(\pi) \varphi_{\sigma}^{\lambda} \varphi_{\pi}^{\lambda} \notag \\
		&= \sum_{\tau \in C_{\sigma t}} \operatorname{sgn}(\pi^{-1} \tau \sigma) \varphi_{\sigma}^{\lambda} \varphi_{\pi^{-1} \tau \sigma}^{\lambda} \notag \\
		&= A_{\sigma t} \varphi_{\sigma}^{\lambda}
	\end{aligned}
	\]
	
\end{document}
